graph/SpaceAdjMatGraph2.v
@@ -101,10 +101,13 @@ Section SpaceAdjMatGraph2.
   Proof.
   Admitted.
 
-  Definition SpaceAdjMatGraph sh (cs: compspecs) (f : E -> E) g gaddr : mpred :=
+  Definition SpaceAdjMatGraph' sh (cs: compspecs) (f : E -> E) g_contents gaddr : mpred :=
     data_at sh (tarray tint (size * size))
-            (map Vint (map Int.repr (graph_to_list g id)))
+            (map Vint (map Int.repr g_contents))
             gaddr.
+
+  Definition SpaceAdjMatGraph sh (cs: compspecs) (f : E -> E) g gaddr : mpred :=
+    SpaceAdjMatGraph' sh cs f (graph_to_list g f) gaddr.
 
 (*
   The below is not currently used by SpaceDijkGraph because 
